Lean4Lean/Theory.lean
@@ -1,1 +1,2 @@
 import Lean4Lean.Theory.Typing.EnvLemmas
+import Lean4Lean.Theory.Typing.Stratified
