Lean4Lean/Theory/Inductive.lean
@@ -2,8 +2,6 @@ import Lean4Lean.Theory.VDecl
 
 namespace Lean4Lean
 
-open Lean (Name FVarId)
-
 def VInductDecl.WF (env : VEnv) (decl : VInductDecl) : Prop := sorry
 
 def VEnv.addInduct (env : VEnv) (decl : VInductDecl) : Option VEnv := sorry
