Lean4Lean/Theory/Typing/InductiveLemmas.lean
@@ -3,10 +3,6 @@ import Lean4Lean.Theory.Typing.Lemmas
 import Lean4Lean.Theory.Typing.Env
 
 namespace Lean4Lean
-
-open Lean (Name FVarId)
-open VExpr
-
 namespace VEnv
 
 theorem addInduct_WF (henv : Ordered env) (hdecl : decl.WF env)
