Lean4Lean/Theory/Typing/Stratified.lean
@@ -1,0 +1,386 @@
+import Lean4Lean.Theory.Typing.Lemmas
+
+namespace Lean4Lean
+namespace VEnv
+
+open VExpr
+
+def DefInv (env : VEnv) (U : Nat) (Γ : List VExpr) : VExpr → VExpr → Prop
+  | .forallE A B, .forallE A' B' =>
+    ∃ u v, env.IsDefEq U Γ A A' (.sort u) ∧ env.IsDefEq U (A::Γ) B B' (.sort v)
+  | .forallE .., .sort .. | .sort .., .forallE .. => False
+  | .sort u, .sort v => u ≈ v
+  | _, _ => True
+
+variable (henv : Ordered env) in
+nonrec theorem DefInv.symm (h : DefInv env U Γ e1 e2) : DefInv env U Γ e2 e1 := by
+  cases e1 <;> cases e2 <;> try trivial
+  · exact h.symm
+  · let ⟨u, v, h1, h2⟩ := h; exact ⟨u, v, h1.symm, h1.defeqDF_l henv h2.symm⟩
+
+section
+set_option hygiene false
+local notation:65 Γ " ⊢ " e " : " A:30 => IsDefEqStrong Γ e e A
+local notation:65 Γ " ⊢ " e1 " ≡ " e2 " : " A:30 => IsDefEqStrong Γ e1 e2 A
+variable (env : VEnv) (uvars : Nat)
+
+inductive IsDefEqStrong : List VExpr → VExpr → VExpr → VExpr → Prop where
+  | bvar : Lookup Γ i A → u.WF uvars → Γ ⊢ A : .sort u → Γ ⊢ .bvar i : A
+  | const :
+    env.constants c = some (some ci) →
+    (∀ l ∈ ls, l.WF uvars) →
+    ls.length = ci.uvars →
+    u.WF uvars →
+    [] ⊢ ci.type.instL ls : .sort u →
+    Γ ⊢ .const c ls : ci.type.instL ls
+  | symm : Γ ⊢ e ≡ e' : A → Γ ⊢ e' ≡ e : A
+  | trans : Γ ⊢ e₁ ≡ e₂ : A → Γ ⊢ e₂ ≡ e₃ : A → Γ ⊢ e₁ ≡ e₃ : A
+  | sortDF :
+    l.WF uvars → l'.WF uvars → l ≈ l' →
+    Γ ⊢ .sort l ≡ .sort l' : .sort (.succ l)
+  | appDF :
+    u.WF uvars → v.WF uvars →
+    Γ ⊢ A : .sort u →
+    A::Γ ⊢ B : .sort v →
+    Γ ⊢ f ≡ f' : .forallE A B →
+    Γ ⊢ a ≡ a' : A →
+    Γ ⊢ B.inst a ≡ B.inst a' : .sort v →
+    Γ ⊢ .app f a ≡ .app f' a' : B.inst a
+  | lamDF :
+    u.WF uvars → v.WF uvars →
+    Γ ⊢ A ≡ A' : .sort u →
+    A::Γ ⊢ B : .sort v →
+    A::Γ ⊢ body ≡ body' : B →
+    Γ ⊢ .lam A body ≡ .lam A' body' : .forallE A B
+  | forallEDF :
+    u.WF uvars → v.WF uvars →
+    Γ ⊢ A ≡ A' : .sort u →
+    A::Γ ⊢ body ≡ body' : .sort v →
+    Γ ⊢ .forallE A body ≡ .forallE A' body' : .sort (.imax u v)
+  | defeqDF :
+    u.WF uvars → Γ ⊢ A ≡ B : .sort u → Γ ⊢ e1 ≡ e2 : A → Γ ⊢ e1 ≡ e2 : B
+  | beta :
+    u.WF uvars → v.WF uvars → Γ ⊢ A : .sort u → A::Γ ⊢ B : .sort v →
+    A::Γ ⊢ e : B → Γ ⊢ e' : A →
+    Γ ⊢ B.inst e' : .sort v →
+    Γ ⊢ e.inst e' : B.inst e' →
+    Γ ⊢ .app (.lam A e) e' ≡ e.inst e' : B.inst e'
+  | eta :
+    u.WF uvars → v.WF uvars → Γ ⊢ A : .sort u → A::Γ ⊢ B : .sort v →
+    Γ ⊢ e : .forallE A B →
+    Γ ⊢ .lam A (.app e.lift (.bvar 0)) ≡ e : .forallE A B
+  | proofIrrel :
+    Γ ⊢ p : .sort .zero → Γ ⊢ h : p → Γ ⊢ h' : p →
+    Γ ⊢ h ≡ h' : p
+  | extra :
+    env.defeqs df → (∀ l ∈ ls, l.WF uvars) → ls.length = df.uvars →
+    u.WF uvars →
+    [] ⊢ df.type.instL ls : .sort u →
+    [] ⊢ df.lhs.instL ls : df.type.instL ls →
+    [] ⊢ df.rhs.instL ls : df.type.instL ls →
+    Γ ⊢ df.lhs.instL ls ≡ df.rhs.instL ls : df.type.instL ls
+
+end
+
+variable (henv : Ordered env) in
+theorem IsDefEqStrong.weakN (W : Ctx.LiftN n k Γ Γ') (H : env.IsDefEqStrong U Γ e1 e2 A) :
+    env.IsDefEqStrong U Γ' (e1.liftN n k) (e2.liftN n k) (A.liftN n k) := by
+  induction H generalizing k Γ' with
+  | bvar h1 h2 h3 => refine .bvar (h1.weakN W) h2 (h3.weakN W)
+  | const h1 h2 h3 h4 h5 =>
+    rw [(henv.closedC h1).instL.liftN_eq (Nat.zero_le _)]
+    exact .const h1 h2 h3 h4 h5
+  | symm _ ih => exact .symm (ih W)
+  | trans _ _ ih1 ih2 => exact .trans (ih1 W) (ih2 W)
+  | sortDF h1 h2 h3 => exact .sortDF h1 h2 h3
+  | appDF h1 h2 _ _ _ _ _ ih1 ih2 ih3 ih4 ih5 =>
+    refine liftN_inst_hi .. ▸ .appDF h1 h2 (ih1 W) (ih2 W.succ) (ih3 W) (ih4 W) ?_
+    exact liftN_inst_hi .. ▸ liftN_inst_hi .. ▸ ih5 W
+  | lamDF h1 h2 _ _ _ ih1 ih2 ih3 => exact .lamDF h1 h2 (ih1 W) (ih2 W.succ) (ih3 W.succ)
+  | forallEDF h1 h2 _ _ ih1 ih2 => exact .forallEDF h1 h2 (ih1 W) (ih2 W.succ)
+  | defeqDF h1 _ _ ih1 ih2 => exact .defeqDF h1 (ih1 W) (ih2 W)
+  | beta h1 h2 _ _ _ _ _ _ ih1 ih2 ih3 ih4 ih5 ih6 =>
+    refine liftN_inst_hi .. ▸ liftN_instN_hi .. ▸ .beta h1 h2
+      (ih1 W) (ih2 W.succ) (ih3 W.succ) (ih4 W)
+      (liftN_instN_hi .. ▸ ih5 W :)
+      (liftN_instN_hi .. ▸ liftN_instN_hi .. ▸ ih6 W :)
+  | eta h1 h2 _ _ _ ih1 ih2 ih3 =>
+    have := IsDefEqStrong.eta h1 h2 (ih1 W) (ih2 W.succ) (ih3 W)
+    simp [liftN]; rwa [← lift_liftN']
+  | proofIrrel _ _ _ ih1 ih2 ih3 => exact .proofIrrel (ih1 W) (ih2 W) (ih3 W)
+  | extra h1 h2 h3 h4 h5 h6 h7 =>
+    have ⟨⟨hA1, _⟩, hA2, hA3⟩ := henv.closed.2 h1
+    rw [
+      hA1.instL.liftN_eq (Nat.zero_le _),
+      hA2.instL.liftN_eq (Nat.zero_le _),
+      hA3.instL.liftN_eq (Nat.zero_le _)]
+    exact .extra h1 h2 h3 h4 h5 h6 h7
+
+theorem IsDefEqStrong.defeq (H : IsDefEqStrong env U Γ e1 e2 A) : env.IsDefEq U Γ e1 e2 A := by
+  induction H with
+  | bvar h => exact .bvar h
+  | const h1 h2 h3 => exact .const h1 h2 h3
+  | symm _ ih => exact .symm ih
+  | trans _ _ ih1 ih2 => exact .trans ih1 ih2
+  | sortDF h1 h2 h3 => exact .sortDF h1 h2 h3
+  | appDF _ _ _ _ _ _ _ _ _ ih1 ih2 => exact .appDF ih1 ih2
+  | lamDF _ _ _ _ _ ih1 _ ih2 => exact .lamDF ih1 ih2
+  | forallEDF _ _ _ _ ih1 ih2 => exact .forallEDF ih1 ih2
+  | defeqDF _ _ _ ih1 ih2 => exact .defeqDF ih1 ih2
+  | beta _ _ _ _ _ _ _ _ _ _ ih1 ih2 => exact .beta ih1 ih2
+  | eta _ _ _ _ _ _ _ ih => exact .eta ih
+  | proofIrrel _ _ _ ih1 ih2 ih3 => exact .proofIrrel ih1 ih2 ih3
+  | extra h1 h2 h3 => exact .extra h1 h2 h3
+
+def CtxStrong (env : VEnv) (U Γ) :=
+  OnCtx Γ fun Γ A => ∃ u, u.WF U ∧ env.IsDefEqStrong U Γ A A (.sort u)
+
+variable (henv : Ordered env) in
+nonrec theorem CtxStrong.lookup {Γ} (H : CtxStrong env U Γ) (h : Lookup Γ i A) :
+    ∃ u, u.WF U ∧ env.IsDefEqStrong U Γ A A (.sort u) :=
+  H.lookup h fun ⟨_, hu, h⟩ => ⟨_, hu, h.weakN henv .one⟩
+
+theorem CtxStrong.defeq {Γ} (H : CtxStrong env U Γ) : OnCtx Γ (env.IsType U) :=
+  H.mono fun ⟨_, _, h⟩ => ⟨_, h.defeq⟩
+
+/-
+variable (henv : Ordered env) (h₀ : env.IsDefEqStrong U Γ₀ e₀ e₀ A₀) (hΓ₀ : CtxStrong env U Γ₀) in
+theorem IsDefEqStrong.instN (W : Ctx.InstN Γ₀ e₀ A₀ k Γ₁ Γ) (H : env.IsDefEqStrong U Γ₁ e1 e2 A)
+    (hΓ : CtxStrong env U Γ) :
+    env.IsDefEqStrong U Γ (e1.inst e₀ k) (e2.inst e₀ k) (A.inst e₀ k) := by
+  induction H generalizing Γ k with
+  | @bvar _ i _ ty h =>
+    dsimp [inst]
+    induction W generalizing i ty with
+    | zero =>
+      cases h with simp [inst_lift]
+      | zero => exact h₀
+      | succ h => let ⟨u, hu, hty⟩ := hΓ₀.lookup henv h; exact .bvar h hu hty
+    | succ _ ih =>
+      cases h with (simp; rw [Nat.add_comm, ← liftN_instN_lo (hj := Nat.zero_le _)])
+      | zero => let ⟨u, hu, hty⟩ := hΓ.lookup henv .zero; exact .bvar .zero hu hty
+      | succ h => exact (ih h _ _).weak henv
+  | const h1 h2 h3 =>
+    rw [(henv.closedC h1).instL.instN_eq (Nat.zero_le _)]
+    exact .const h1 h2 h3
+  | symm _ ih => exact .symm (ih W)
+  | trans _ _ ih1 ih2 => exact .trans (ih1 W) (ih2 W)
+  | sortDF h1 h2 h3 => exact .sortDF h1 h2 h3
+  | appDF _ _ ih1 ih2 => exact inst_inst_hi .. ▸ .appDF (ih1 W) (ih2 W)
+  | lamDF _ _ ih1 ih2 => exact .lamDF (ih1 W) (ih2 W.succ)
+  | forallEDF _ _ ih1 ih2 => exact .forallEDF (ih1 W) (ih2 W.succ)
+  | defeqDF _ _ ih1 ih2 => exact .defeqDF (ih1 W) (ih2 W)
+  | beta _ _ ih1 ih2 =>
+    exact inst_inst_hi .. ▸ inst_inst_hi .. ▸ .beta (ih1 W.succ) (ih2 W)
+  | @eta _ e A B _ ih =>
+    have := IsDefEq.eta (ih W)
+    rw [lift, liftN_instN_lo (hj := Nat.zero_le _), Nat.add_comm] at this
+    simpa [inst]
+  | proofIrrel _ _ _ ih1 ih2 ih3 => exact .proofIrrel (ih1 W) (ih2 W) (ih3 W)
+  | extra h1 h2 h3 =>
+    have ⟨⟨hA1, _⟩, hA2, hA3⟩ := henv.closed.2 h1
+    rw [
+      hA1.instL.instN_eq (Nat.zero_le _),
+      hA2.instL.instN_eq (Nat.zero_le _),
+      hA3.instL.instN_eq (Nat.zero_le _)]
+    exact .extra h1 h2 h3
+
+variable (henv : Ordered env) in
+theorem IsDefEq.strong'
+    (envIH : env.OnTypes fun U e A => env.IsDefEqStrong U [] e e A ∧ env.IsType U [] A)
+    (hΓ : CtxStrong env U Γ)
+    (H : env.IsDefEq U Γ e1 e2 A) :
+    env.IsDefEqStrong U Γ e1 e2 A := by
+  have hctx {Γ} (H : OnCtx Γ fun Γ A => ∃ u, u.WF U ∧ env.IsDefEqStrong U Γ A A (.sort u)) :
+     OnCtx Γ (env.IsType U) := H.mono fun ⟨_, _, h⟩ => ⟨_, h.defeq⟩
+  induction H with
+  | bvar h =>
+    let ⟨u, hu, hA⟩ := hΓ.lookup h fun ⟨u, hu, h⟩ => ⟨_, hu, h.weakN henv .one⟩
+    exact .bvar h (hA.defeq.sort_r henv (hctx hΓ)) hA
+  | @const _ _ ls' _ h1 h2 h3 =>
+    refine' .const h1 h2 h3 _ _
+    refine ⟨.const h1 h2 h3, .const h1 h2 h3, .refl <| hty <| .const h1 h2 h3⟩
+  | symm _ ih =>
+    -- let ⟨ty1, ty2, df⟩ := ih
+    exact ⟨ty2, ty1, .symm df⟩
+  | trans _ _ ih1 ih2 =>
+    -- let ⟨ty1, ty2, df1⟩ := ih1; let ⟨_, ty3, df2⟩ := ih2
+    exact ⟨ty1, ty3, .trans df1 df2⟩
+  | sortDF h1 h2 h3 =>
+    refine ⟨.sort h1, .defeq (hdf ?_) (.sort h2), .sortDF h1 h2 h3⟩
+    exact .symm <| .sortDF h1 h2 <| VLevel.succ_congr h3
+  | appDF _ _ ih1 ih2 =>
+    -- let ⟨hf, hf', ff⟩ := ih1; let ⟨ha, ha', aa⟩ := ih2
+    refine' ⟨.app hf ha, .defeq (hdf (.instDF hB _ _ _ _ _)) (.app hf' ha'),
+      .appDF (hty hf) (hty hf') (hty ha) (hty ha') ff aa⟩
+
+    exact instL_instN ▸ .appDF ih1 ih2
+  | lamDF _ _ ih1 ih2 => exact .lamDF ih1 ih2
+  | forallEDF _ _ ih1 ih2 => exact .forallEDF ih1 ih2
+  | defeqDF _ _ ih1 ih2 => exact .defeqDF ih1 ih2
+  | beta _ _ ih1 ih2 => sorry
+  | eta _ ih => sorry
+  | proofIrrel _ _ _ ih1 ih2 ih3 => exact .proofIrrel ih1 ih2 ih3
+  | extra h1 h2 h3 =>
+    simp [instL, instL_instL]
+    exact .extra h1 (by simp [h2, VLevel.WF.inst hls]) (by simp [h3])
+
+section
+set_option hygiene false
+local notation:65 Γ " ⊢ " e " : " A:30 => HasType1 Γ e A
+local notation:65 Γ " ⊢ " e1 " ≡ " e2:30 => IsDefEq1 Γ e1 e2
+
+variable (env : VEnv) (uvars : Nat)
+
+variable (IsDefEq1 : List VExpr → VExpr → VExpr → Prop) in
+inductive HasType1 : List VExpr → VExpr → VExpr → Prop where
+  | bvar : Lookup Γ i A → Γ ⊢ .bvar i : A
+  | const :
+    env.constants c = some (some ci) →
+    (∀ l ∈ ls, l.WF uvars) →
+    ls.length = ci.uvars →
+    Γ ⊢ .const c ls : ci.type.instL ls
+  | sort : l.WF uvars → Γ ⊢ .sort l : .sort (.succ l)
+  | app : Γ ⊢ f : .forallE A B → Γ ⊢ a : A → Γ ⊢ .app f a : B.inst a
+  | lam : Γ ⊢ A : .sort u → A::Γ ⊢ body : B → Γ ⊢ .lam A body : .forallE A B
+  | forallE : Γ ⊢ A : .sort u → A::Γ ⊢ body : .sort v → Γ ⊢ .forallE A body : .sort (.imax u v)
+  | defeq : Γ ⊢ A ≡ B → Γ ⊢ e : A → Γ ⊢ e : B
+  | inst : A::Γ ⊢ e : B → Γ ⊢ e' : A → Γ ⊢ e.inst e' : B.inst e'
+
+variable (HasType1 : List VExpr → VExpr → VExpr → Prop) in
+inductive IsDefEq1 : List VExpr → VExpr → VExpr → Prop where
+  | refl : Γ ⊢ e : A → Γ ⊢ e ≡ e
+  | symm : Γ ⊢ e ≡ e' → Γ ⊢ e' ≡ e
+  | trans : Γ ⊢ e₁ ≡ e₂ → Γ ⊢ e₂ ≡ e₃ → Γ ⊢ e₁ ≡ e₃
+  | sortDF : l.WF uvars → l'.WF uvars → l ≈ l' → Γ ⊢ .sort l ≡ .sort l'
+  | appDF :
+    Γ ⊢ f : .forallE A B → Γ ⊢ f' : .forallE A B → Γ ⊢ a : A → Γ ⊢ a' : A →
+    Γ ⊢ f ≡ f' → Γ ⊢ a ≡ a' → Γ ⊢ .app f a ≡ .app f' a'
+  | lamDF : Γ ⊢ A ≡ A' → A::Γ ⊢ B ≡ B' → Γ ⊢ .lam A B ≡ .lam A' B'
+  | forallEDF : Γ ⊢ A ≡ A' → A::Γ ⊢ B ≡ B' → Γ ⊢ .forallE A B ≡ .forallE A' B'
+  | instDF :
+    A::Γ ⊢ f : B → A::Γ ⊢ f' : B → Γ ⊢ a : A → Γ ⊢ a' : A →
+    Γ ⊢ f ≡ f' → Γ ⊢ a ≡ a' → Γ ⊢ .inst f a ≡ .inst f' a'
+  | beta : A::Γ ⊢ e : B → Γ ⊢ e' : A → Γ ⊢ .app (.lam A e) e' ≡ e.inst e'
+  | eta : Γ ⊢ e : .forallE A B → Γ ⊢ .lam A (.app e.lift (.bvar 0)) ≡ e
+  | proofIrrel : Γ ⊢ p : .sort .zero → Γ ⊢ h : p → Γ ⊢ h' : p → Γ ⊢ h ≡ h'
+  | extra :
+    env.defeqs df → (∀ l ∈ ls, l.WF uvars) → ls.length = df.uvars →
+    Γ ⊢ df.lhs.instL ls ≡ df.rhs.instL ls
+
+end
+
+theorem IsDefEq.induction1
+    (defEq : List VExpr → VExpr → VExpr → Prop)
+    (hasType : List VExpr → VExpr → VExpr → Prop)
+    (hty : ∀ {Γ e A}, HasType1 env U defEq Γ e A → hasType Γ e A)
+    (hdf : ∀ {Γ e1 e2}, IsDefEq1 env U hasType Γ e1 e2 → defEq Γ e1 e2)
+    (H : env.IsDefEq U Γ e1 e2 A) :
+    HasType1 env U defEq Γ e1 A ∧
+    HasType1 env U defEq Γ e2 A ∧
+    IsDefEq1 env U hasType Γ e1 e2 := by
+  induction H with
+  | bvar h => exact ⟨.bvar h, .bvar h, .refl (hty (.bvar h))⟩
+  | @const _ _ ls' _ h1 h2 h3 =>
+    refine ⟨.const h1 h2 h3, .const h1 h2 h3, .refl <| hty <| .const h1 h2 h3⟩
+  | symm _ ih =>
+    let ⟨ty1, ty2, df⟩ := ih
+    exact ⟨ty2, ty1, .symm df⟩
+  | trans _ _ ih1 ih2 =>
+    let ⟨ty1, ty2, df1⟩ := ih1; let ⟨_, ty3, df2⟩ := ih2
+    exact ⟨ty1, ty3, .trans df1 df2⟩
+  | sortDF h1 h2 h3 =>
+    refine ⟨.sort h1, .defeq (hdf ?_) (.sort h2), .sortDF h1 h2 h3⟩
+    exact .symm <| .sortDF h1 h2 <| VLevel.succ_congr h3
+  | appDF _ _ ih1 ih2 =>
+    let ⟨hf, hf', ff⟩ := ih1; let ⟨ha, ha', aa⟩ := ih2
+    refine' ⟨.app hf ha, .defeq (hdf (.instDF hB _ _ _ _ _)) (.app hf' ha'),
+      .appDF (hty hf) (hty hf') (hty ha) (hty ha') ff aa⟩
+
+    exact instL_instN ▸ .appDF ih1 ih2
+  | lamDF _ _ ih1 ih2 => exact .lamDF ih1 ih2
+  | forallEDF _ _ ih1 ih2 => exact .forallEDF ih1 ih2
+  | defeqDF _ _ ih1 ih2 => exact .defeqDF ih1 ih2
+  | beta _ _ ih1 ih2 => simpa using .beta ih1 ih2
+  | eta _ ih => simpa [instL] using .eta ih
+  | proofIrrel _ _ _ ih1 ih2 ih3 => exact .proofIrrel ih1 ih2 ih3
+  | extra h1 h2 h3 =>
+    simp [instL, instL_instL]
+    exact .extra h1 (by simp [h2, VLevel.WF.inst hls]) (by simp [h3])
+
+
+
+variable (henv : Ordered env) in
+theorem IsDefEq.unique_typing'
+    (H1 : env.IsDefEq U Γ e1 e2 A1) (H2 : env.IsDefEq U Γ e1 e2 A2) :
+    ∃ u, env.IsDefEq U Γ A1 A2 (.sort u) := by
+  generalize eq1 : e1 = e1', eq2 : e2 = e2' at H2
+  induction H1 generalizing A2 with
+  | bvar h =>
+
+    refine .bvar h.instL
+  | @const _ _ ls' _ h1 h2 h3 =>
+    simp [instL, instL_instL]
+    exact .const h1 (by simp [h2, VLevel.WF.inst hls]) (by simp [h3])
+  | symm _ ih => exact .symm ih
+  | trans _ _ ih1 ih2 => exact .trans ih1 ih2
+  | sortDF _ _ h3 =>
+    exact .sortDF (VLevel.WF.inst hls) (VLevel.WF.inst hls) (VLevel.inst_congr_l h3)
+  | appDF _ _ ih1 ih2 => exact instL_instN ▸ .appDF ih1 ih2
+  | lamDF _ _ ih1 ih2 => exact .lamDF ih1 ih2
+  | forallEDF _ _ ih1 ih2 => exact .forallEDF ih1 ih2
+  | defeqDF _ _ ih1 ih2 => exact .defeqDF ih1 ih2
+  | beta _ _ ih1 ih2 => simpa using .beta ih1 ih2
+  | eta _ ih => simpa [instL] using .eta ih
+  | proofIrrel _ _ _ ih1 ih2 ih3 => exact .proofIrrel ih1 ih2 ih3
+  | extra h1 h2 h3 =>
+    simp [instL, instL_instL]
+    exact .extra h1 (by simp [h2, VLevel.WF.inst hls]) (by simp [h3])
+-/
+
+
+/- depends on church-rosser
+variable {env : VEnv} (henv : env.Ordered) in
+theorem IsDefEq.weakN_inv (W : Ctx.LiftN n k Γ Γ')
+    (H : env.IsDefEq U Γ' (e1.liftN n k) (e2.liftN n k) (A.liftN n k)) :
+    env.IsDefEq U Γ e1 e2 A := by
+  generalize eq1 : e1.liftN n k = e1', eq2 : e2.liftN n k = e2', eqA : A.liftN n k = A' at H
+  induction H generalizing k e1 e2 A with
+  | bvar h =>
+    cases eqA; cases e1 <;> cases eq1; cases e2 <;> injection eq2
+    cases liftVar_inj.1 ‹_›; exact .bvar (h.weakN_inv W)
+  | @const c ci ls Γ h1 h2 h3 =>
+    cases e1 <;> cases eq1; cases e2 <;> cases eq2
+    rw [ClosedN.liftN_eq_rev (eqA ▸ (henv.closedC h1).instL) (Nat.zero_le _)] at eqA
+    exact eqA ▸ .const h1 h2 h3
+  | symm _ ih => exact .symm (ih W eq2 eq1 eqA)
+  | trans _ _ ih1 ih2 => sorry
+  -- | sortDF h1 h2 h3 => exact .sortDF h1 h2 h3
+  -- | appDF _ _ ih1 ih2 => exact liftN_inst_hi .. ▸ .appDF (ih1 W) (ih2 W)
+  -- | lamDF _ _ ih1 ih2 => exact .lamDF (ih1 W) (ih2 W.succ)
+  -- | forallEDF _ _ ih1 ih2 => exact .forallEDF (ih1 W) (ih2 W.succ)
+  -- | defeqDF _ _ ih1 ih2 => exact .defeqDF (ih1 W) (ih2 W)
+  -- | beta _ _ ih1 ih2 =>
+  --   exact liftN_inst_hi .. ▸ liftN_instN_hi .. ▸ .beta (ih1 W.succ) (ih2 W)
+  -- | eta _ ih =>
+  --   have := IsDefEq.eta (ih W)
+  --   simp [liftN]; rwa [← lift_liftN']
+  -- | proofIrrel _ _ _ ih1 ih2 ih3 => exact .proofIrrel (ih1 W) (ih2 W) (ih3 W)
+  -- | extra h1 h2 h3 =>
+  --   have ⟨⟨hA1, _⟩, hA2, hA3⟩ := henv.closed.2 h1
+  --   rw [
+  --     hA1.instL.liftN_eq (Nat.zero_le _),
+  --     hA2.instL.liftN_eq (Nat.zero_le _),
+  --     hA3.instL.liftN_eq (Nat.zero_le _)]
+  --   exact .extra h1 h2 h3
+  | _ => sorry
+
+variable {env : VEnv} (henv : env.Ordered) in
+theorem HasType.weakN_inv (W : Ctx.LiftN n k Γ Γ')
+    (H : env.HasType U Γ' (e.liftN n k) (A.liftN n k)) :
+    env.HasType U Γ e A := IsDefEq.weakN_inv henv W H
+
+variable {env : VEnv} (henv : env.Ordered) in
+theorem IsType.weakN_inv (W : Ctx.LiftN n k Γ Γ') (H : env.IsType U Γ' (A.liftN n k)) :
+    env.IsType U Γ A := let ⟨_, h⟩ := H; ⟨_, h.weakN_inv henv W⟩
+-/
